\begin{problem}
    Let $M$ be a finitely generated $A$-module and let $S \subseteq A$ be a multiplicatively closed set.
    Prove that $S^{-1}M = 0$ if and only if there exists $s \in S$ such that $sM = 0$.
    \begin{sol}
        \begin{proof}
            Take $a_1, \dots, a_n$ an $A$-system of generators of $M$.
            We will prove both implications:
            \begin{itemize}
                \item[$(\Rightarrow)$]
                \begin{claim}
                    If $S^{-1}M = 0$, then for all $a \in M$ there exists some $t \in S$ such that $t a = 0$.
                    \begin{proof}
                        Take $a \in M$ and $s \in S$.
                        Because of the condition, $\frac{a}{s} = \frac{0}{1}$
                        so, for some $t \in S$, $ta = t (a 1 - 0 s) = 0$.
                    \end{proof}
                \end{claim}
                Because of the claim we have that there exist $t_1, \dots, t_n \in S$ such that \linebreak
                ${t_1 a_1 = \cdots = t_n a_n = 0}$.
                Take their product $t = t_1 \dots t_n \in S$.
                We have that for all $m = c_1 a_1 + \dots + c_n a_n \in M$ with $c_1, \dots, c_n \in A$,
                \[
                    t m = c_1 (t a_1) + \dots + c_n (t a_n) = 0
                \]

                \item[$(\Leftarrow)$]
                By hypothesis, there exists $s \in S$ such that $s a = 0$ for all $a \in A$.
                Now, take ${m = \frac{a'}{s'} \in S^{-1}M}$ with $a' \in M$ and $s \in S$.
                We have that $0 = s a' = s (a' 1 - 0 s')$ and thus $m = \frac{a'}{s'} = \frac{0}{1} = 0$.
            \end{itemize}
        \end{proof}
    \end{sol}
\end{problem}