\begin{problem}
    Compute the following:

    \begin{enumerate}[label=(\theproblem.\arabic*),ref=\theproblem.\arabic*]
        \item $\text{Hom}_{\mathbb{Z}}(\mathbb{Q}, \mathbb{Z})$:
        \begin{sol}
            Suppose $\varphi$ is one such homomorphism.
            Let $n = \varphi\left(\frac{a}{b}\right)$.
            If $n \neq 0$, then $n = \varphi\left(\frac{2na}{2nb}\right) = (2n)\varphi\left(\frac{a}{2nb}\right) \Rightarrow 2n \mid n$, a contradiction.
            Therefore, $\text{Hom}_{\mathbb{Z}}(\mathbb{Q}, \mathbb{Z}) = \{0\}$.
        \end{sol}

        \item $\text{Hom}_{\mathbb{Z}}(\mathbb{Q}, \mathbb{Q})$:
            \begin{sol}
                Suppose $\varphi$ is one such homomorphism.
                Let $\varphi(1) = h$.
                Then, for all fractions of the form $\frac{p}{q}$,
                $q\varphi\left(\frac{p}{q}\right) = pq \varphi\left(\frac{1}{q}\right) = p f\left(\frac{q}{q}\right) = ph \Rightarrow
                f\left(\frac{p}{q}\right) = \frac{p}{q}h$.
                Therefore, we get a homomorphism $\varphi_h$ corresponding to each $h\in \mathbb{Q}$, consisting in multiplying by it.
                Indeed, all of these are $\mathbb{Z}$-module homomorphisms:
                \begin{itemize}
                    \item $\varphi_h(nf) = h(nf) = n(hf) = n\varphi_h(f)$.
                    \item $\varphi_h(f+g) = h(f+g) = hf + hg = \varphi_h(f) + \varphi_h(g)$.
                \end{itemize}
                And they are all different, since $\varphi_h(1) = h$.
            \end{sol}
        \item $\text{Hom}_{\mathbb{Z}}(\mathbb{Z}/(m), \mathbb{Q})$:
            \begin{sol}
                Suppose $\varphi$ is one such homomorphism.
                Let $x \in \mathbb{Z}/(m)$.
                Then, 0 = $\varphi(0) = \varphi(m \cdot x) = m\cdot \varphi(x) = \frac{m}{1}\varphi(x) \Rightarrow \varphi(x) = 0$.
                Therefore, $\text{Hom}_{\mathbb{Z}}(\mathbb{Z}/(m), \mathbb{Q}) = \{0\}$.

            \end{sol}
    \end{enumerate}
\end{problem}